@prefix dc: <http://purl.org/dc/terms/> .
@prefix owl: <http://www.w3.org/2002/07/owl#> .
@prefix rdf: <http://www.w3.org/1999/02/22-rdf-syntax-ns#> .
@prefix xml: <http://www.w3.org/XML/1998/namespace> .
@prefix xsd: <http://www.w3.org/2001/XMLSchema#> .
@prefix foaf: <http://xmlns.com/foaf/0.1/> .
@prefix rdfs: <http://www.w3.org/2000/01/rdf-schema#> .
@prefix skos: <http://www.w3.org/2004/02/skos/core#> .

@base <https://simonkjohnston.life/ontology/2022/parthood.ttl> .
@prefix : <https://simonkjohnston.life/ontology/2022/parthood.ttl#> .

:   a owl:Ontology ;
    owl:versionInfo "0.1.0" ;
    owl:versionIRI <https://simonkjohnston.life/ontology/2022/parthood/1.0.0> ;
    dc:issued "2022-08-06"^^xsd:date ;
    dc:identifier "parthood.ttl" ;
    
    skos:prefLabel "Simple Parthood Ontology"@en ;
    dc:description "A simple mereological ontology that models simple part/whole relations. Note that this also recognizes the difference between parts, components, and constituents of a whole."@en ;
    rdfs:seeAlso <https://plato.stanford.edu/entries/mereology/> ;
    dc:creator [
        foaf:mbox "johnstonskj@gmail.com" ;
        foaf:name "Simon Johnston"
    ] .

#################################################################
#    Object Properties
#################################################################

:componentOf
    rdf:type
        owl:ObjectProperty ,
        owl:AsymmetricProperty ,
        owl:TransitiveProperty ,
        owl:ReflexiveProperty ;
    owl:inverseOf :hasComponent ;
    rdfs:domain :component ;
    rdfs:isDefinedBy <https://simonkjohnston.life/ontology/2022/parthood/0.1.0> ;
    
    skos:definition "hasComponent and componentOf represent a non-strict partial ordering, a reflexive and anti-symmetric relation relating components."@en ;
    skos:prefLabel "component-of" .


:constituentOf
    rdf:type
        owl:ObjectProperty ,
        owl:AsymmetricProperty ,
        owl:TransitiveProperty ,
        owl:ReflexiveProperty ;
    owl:inverseOf :hasConstituent ;
    rdfs:domain :constituent ;
    rdfs:isDefinedBy <https://simonkjohnston.life/ontology/2022/parthood/0.1.0> ;

    skos:definition "hasConstituent and constituentOf represent a non-strict partial ordering, a reflexive and anti-symmetric relation relating constituents."@en ;
    skos:prefLabel "constituent-of" .


:hasComponent
    rdf:type
        owl:ObjectProperty ,
        owl:AsymmetricProperty ,
        owl:TransitiveProperty ,
        owl:ReflexiveProperty ;
    rdfs:range :component ;
    rdfs:isDefinedBy <https://simonkjohnston.life/ontology/2022/parthood/0.1.0> ;

    skos:definition "hasComponent and componentOf represent a non-strict partial ordering, a reflexive and anti-symmetric relation relating components."@en ;
;74;43M    skos:prefLabel "has component" .


:hasConstituent
    rdf:type
        owl:ObjectProperty ,
        owl:AsymmetricProperty ,
        owl:TransitiveProperty ,
        owl:ReflexiveProperty ;
    rdfs:range :constituent ;
    rdfs:isDefinedBy <https://simonkjohnston.life/ontology/2022/parthood/0.1.0> ;

    skos:definition "hasConstituent and constituentOf represent a non-strict partial ordering, a reflexive and anti-symmetric relation relating constituents."@en ;
    skos:prefLabel "has constituent" .


:hasPart
    rdf:type
        owl:ObjectProperty ,
        owl:AsymmetricProperty ,
        owl:TransitiveProperty ,
        owl:ReflexiveProperty ;
    owl:inverseOf :partOf ;
    rdfs:range :part ;
    rdfs:isDefinedBy <https://simonkjohnston.life/ontology/2022/parthood/0.1.0> ;

    skos:definition "hasPart and partOf represent a non-strict partial ordering, a reflexive and anti-symmetric relation relating parts."@en ;
    skos:prefLabel "has part" .


:hasProperComponent
    rdf:type
        owl:ObjectProperty ,
        owl:AsymmetricProperty ,
        owl:TransitiveProperty ,
        owl:IrreflexiveProperty ;
    owl:inverseOf :properComponentOf ;
    rdfs:range :component ;
    rdfs:isDefinedBy <https://simonkjohnston.life/ontology/2022/parthood/0.1.0> ;

    skos:definition "hasProperComponent and properComponentOf represent a strict partial ordering, an irreflexive and anti-symmetric relation relating components."@en ;
    skos:prefLabel "has proper component" .


:hasProperConstituent
    rdf:type
        owl:ObjectProperty ,
        owl:AsymmetricProperty ,
        owl:TransitiveProperty ,
        owl:IrreflexiveProperty ;
    owl:inverseOf :properConstituentOf ;
    rdfs:range :constituent ;
    rdfs:isDefinedBy <https://simonkjohnston.life/ontology/2022/parthood/0.1.0> ;

    skos:definition "hasProperConstituent and properConstituentOf represent a strict partial ordering, an irreflexive and anti-symmetric relation relating constituents."@en ;
    skos:prefLabel "has proper constituent" .


:hasProperPart
    rdf:type
        owl:ObjectProperty ,
        owl:AsymmetricProperty ,
        owl:TransitiveProperty ,
        owl:IrreflexiveProperty ;
    owl:inverseOf :properPartOf ;
    rdfs:range :part ;
    rdfs:isDefinedBy <https://simonkjohnston.life/ontology/2022/parthood/0.1.0> ;

    skos:definition "hasProperPart and properPartOf represent a strict partial ordering, an irreflexive and anti-symmetric relation relating parts."@en ;
    skos:prefLabel "has proper part" .


:partOf
    rdf:type
        owl:ObjectProperty ,
        owl:AsymmetricProperty ,
        owl:TransitiveProperty ,
        owl:ReflexiveProperty ;
    rdfs:domain :part ;
    rdfs:isDefinedBy <https://simonkjohnston.life/ontology/2022/parthood/0.1.0> ;

    skos:definition "hasPart and partOf represent a non-strict partial ordering, a reflexive and anti-symmetric relation relating parts."@en ;
    skos:prefLabel "part-of" .


:properComponentOf
    rdf:type
        owl:ObjectProperty ,
        owl:AsymmetricProperty ,
        owl:TransitiveProperty ,
        owl:IrreflexiveProperty ;
    rdfs:domain :component ;
    rdfs:isDefinedBy <https://simonkjohnston.life/ontology/2022/parthood/0.1.0> ;

    skos:definition "hasProperComponent and properComponentOf represent a strict partial ordering, an irreflexive and anti-symmetric relation relating components."@en ;
    skos:prefLabel "proper component-of" .


:properConstituentOf
    rdf:type
        owl:ObjectProperty ,
        owl:AsymmetricProperty ,
        owl:TransitiveProperty ,
        owl:IrreflexiveProperty ;
    rdfs:domain :constituent ;
    rdfs:isDefinedBy <https://simonkjohnston.life/ontology/2022/parthood/0.1.0> ;

    skos:definition "hasProperConstituent and properConstituentOf represent a strict partial ordering, an irreflexive and anti-symmetric relation relating constituents."@en ;
    skos:prefLabel "proper constituent-of" .


:properPartOf
    rdf:type
        owl:ObjectProperty ,
        owl:AsymmetricProperty ,
        owl:TransitiveProperty ,
        owl:IrreflexiveProperty ;
    rdfs:domain :part ;
    rdfs:isDefinedBy <https://simonkjohnston.life/ontology/2022/parthood/0.1.0> ;

    skos:definition "hasProperPart and properPartOf represent a strict partial ordering, an irreflexive and anti-symmetric relation relating parts."@en ;
    skos:prefLabel "proper part-of" .


#################################################################
#    Classes
#################################################################

:atom
    rdf:type owl:Class ;
    rdfs:isDefinedBy <https://simonkjohnston.life/ontology/2022/parthood/0.1.0> ;

    skos:definition "Some object that has no identifiable parts."@en ;
    skos:prefLabel "Atom"@en .


:component
    rdf:type owl:Class ;
    rdfs:subClassOf
        :part,
        :whole ;
    owl:disjointWith :constituent ;
    rdfs:isDefinedBy <https://simonkjohnston.life/ontology/2022/parthood/0.1.0> ;

    skos:definition "A kind of part which has it's own identity as a whole in some context."@en ;
    skos:prefLabel "Component"@en .


:constituent
    rdf:type owl:Class ;
    rdfs:subClassOf :part ;
    owl:disjointWith :component ;
    rdfs:isDefinedBy <https://simonkjohnston.life/ontology/2022/parthood/0.1.0> ;

    skos:definition "A kind of part that, when described as a part of the whole, is no longer identifiable."@en ;
    skos:prefLabel "Constituent"@en .


:part
    rdf:type owl:Class ;
    rdfs:isDefinedBy <https://simonkjohnston.life/ontology/2022/parthood/0.1.0> ;

    skos:definition "Some object that is a part, in a broad mereological term, of some whole."@en ;
    skos:prefLabel "Part"@en .


:whole
    rdf:type owl:Class ;
    rdfs:isDefinedBy <https://simonkjohnston.life/ontology/2022/parthood/0.1.0> ;

    skos:definition "Some object that is made of parts."@en ;
    skos:prefLabel "Whole"@en .
